Added coke machine and dining philosophers exercises and slightly modified other files in chapter 3

chapter03/exercises/exercise04.dfy
@@ -32,19 +32,3 @@ predicate Next(s:State, s':State) {
 predicate Safety(s:State) {
   true  // Change me to the important property!
 }
-
-predicate Inv(s: State) {
-  Safety(s)
-}
-
-// This is the boilerplate proof obligation you might like. For this exercise,
-// focus on modeling the system described above with a state machine and
-// *stating* a safety property; don't try to prove the safety property yet.
-// We'll prove it in chapter04/exercise02.
-//
-// lemma SafetyProof()
-//   ensures forall s :: Init(s) ==> Inv(s)
-//   ensures forall s, s' :: Inv(s) && Next(s, s') ==> Inv(s')
-//   ensures forall s :: Inv(s) ==> Safety(s)
-// {
-// }
