chapter03/demos/demo01.dfy
@@ -1,3 +1,8 @@
+//#instructor The switch is an example of a very simple state machine.
+//#instructor All its steps are non-parameterized.
+//#instructor This example is intended to show the basic of the boilerplate
+//#instructor of a TLA+ state machine embedded in Dafny.
+
 datatype SwitchState = On | Off
 
 datatype State = State(switch:SwitchState)
