chapter03/demos/exercise01.dfy
@@ -1,0 +1,71 @@
+//#instructor This is the first state machine specification example.
+//#instructor Its complexity is about the same as the library. We 
+//#instructor provide the boilerplate for everything, but leave the state
+//#instructor transitions as an exercise.
+//#instructor It comes with a safety proof that we expect the students to use as an 
+//#instructor oracle for whether they got the state transitions right.
+
+datatype CokeMachine = CokeMachine(numCokes:int)
+
+function maxCokes() : int {
+   7
+} 
+
+predicate Init(cm:CokeMachine) {
+    cm.numCokes == 0
+}
+
+predicate Purchase(cm:CokeMachine, cm':CokeMachine) {
+//#elide    && cm.numCokes > 0
+//#elide    && cm'.numCokes == cm.numCokes - 1
+}
+
+predicate Restock(cm:CokeMachine, cm':CokeMachine, numRestock:int) 
+{
+//#elide    && numRestock >= 0
+//#elide    && cm.numCokes + numRestock <= maxCokes()
+//#elide    && cm'.numCokes == cm.numCokes + numRestock
+}
+
+predicate Next(cm:CokeMachine, cm':CokeMachine) {
+    || Purchase(cm, cm')
+    || (exists n :: Restock(cm, cm', n))
+} 
+
+//==========================
+predicate Inv(cm:CokeMachine) {
+    0 <= cm.numCokes <= maxCokes()
+}
+
+lemma SafetyProof() 
+    ensures forall cm | Init(cm) :: Inv(cm)
+    ensures forall cm, cm' | Inv(cm) && Next(cm, cm') :: Inv(cm')
+{
+    forall cm, cm' | Inv(cm) && Next(cm, cm') 
+        ensures Inv(cm')
+    {
+        if(Purchase(cm, cm')) {
+            assert Inv(cm');
+        } else {
+            var n :| Restock(cm, cm', n);
+            assert Inv(cm');
+        }   
+    }
+}
+
+lemma NonTrivialPurchase()
+    ensures exists cm, cm' :: Inv(cm) && Next(cm, cm') && cm'.numCokes + 1 == cm.numCokes
+{
+    var cm := CokeMachine(1);   
+    var cm' := CokeMachine(0);   
+    assert Inv(cm) && Next(cm, cm') && cm'.numCokes + 1 == cm.numCokes;
+}
+
+lemma NonTrivialRestock()
+    ensures exists cm, cm' :: Inv(cm) && Next(cm, cm') && cm.numCokes < cm'.numCokes
+{
+    var cm := CokeMachine(4);   
+    var cm' := CokeMachine(7);   
+    assert Restock(cm, cm', 3);
+    assert Inv(cm) && Next(cm, cm') && cm.numCokes < cm'.numCokes;
+}
