chapter03/demos/exercise02.dfy
@@ -1,0 +1,119 @@
+//#instructor 
+//#instructor 
+//#instructor Relative to the coke machine, the students need to
+//#instructor write their own datatype for philosophers and pair
+//#instructor (or equivalent concepts)
+//#instructor Introduces the constants idiom.
+//#instructor 
+
+
+datatype Constants = Constants(tableSize:nat)
+
+//#elide datatype Pair = Pair(left:bool, right:bool)
+datatype State = State(
+//#elide     philosophers:seq<Pair>
+)
+
+predicate WellFormedConstants(c:Constants) {
+    && 0 < c.tableSize 
+}
+
+predicate WellFormed(c:Constants, s:State) {
+    && WellFormedConstants(c)
+//#elide    && |s.philosophers| == c.tableSize
+}
+
+predicate Init(c:Constants, s:State) {
+//#elide    && WellFormed(c, s)
+//#elide    && (forall pi | 0 <= pi < |s.philosophers| :: s.philosophers[pi] == Pair(false, false))
+}
+
+predicate AcquireLeft(c:Constants, s:State, s':State, pi:nat) {
+//#elide    && WellFormed(c, s)
+//#elide    && pi < c.tableSize
+//#elide    && !(s.philosophers[pi].left) // prevents this action from being a no-op
+//#elide    && !(s.philosophers[PhilosopherToTheLeftOf(c,pi)].right) // comment this line to create bug
+//#elide    && s' == s.(philosophers := s.philosophers[pi := Pair(true, s.philosophers[pi].right)])
+}
+
+predicate AcquireRight(c:Constants, s:State, s':State, pi:nat) {
+//#elide    && WellFormed(c, s)
+//#elide    && pi < c.tableSize
+//#elide    && !(s.philosophers[pi].right) // prevents this action from being a no-op
+//#elide    && !(s.philosophers[PhilosopherToTheRightOf(c,pi)].left) // comment this line to create bug
+//#elide    && s' == s.(philosophers := s.philosophers[pi := Pair(s.philosophers[pi].left, true)])
+}
+
+predicate ReleaseBoth(c:Constants, s:State, s':State, pi:nat) {
+//#elide    && WellFormed(c, s)
+//#elide    && pi < c.tableSize
+//#elide    && (s.philosophers[pi].left)
+//#elide    && (s.philosophers[pi].right)
+//#elide    && s' == s.(philosophers := s.philosophers[pi := Pair(false, false)])
+}
+ 
+function PhilosopherToTheLeftOf(c:Constants, i:nat) : nat 
+    requires WellFormedConstants(c)
+{
+    (i+1) % c.tableSize
+}
+
+function PhilosopherToTheRightOf(c:Constants, i:nat) : nat 
+    requires WellFormedConstants(c)
+{
+    (i-1) % c.tableSize
+}
+
+predicate Next(c:Constants, s:State, s':State) {
+//#elide    exists pi:nat :: 
+//#elide    (|| AcquireLeft(c, s, s', pi)
+//#elide     || AcquireRight(c, s, s', pi)
+//#elide     || ReleaseBoth(c, s, s', pi))
+}
+
+// here is the safety property
+predicate ForkConsistency(c:Constants, s:State) 
+{
+    && WellFormed(c, s)
+    && (forall i | 0 <= i < c.tableSize :: !(
+        && s.philosophers[i].right 
+        && s.philosophers[PhilosopherToTheRightOf(c,i)].left
+        ))
+}
+
+// here is a proof of the safety property. This lemma should verify
+// without adding a body 
+lemma ForkConsistencyLemma() 
+    ensures forall c, s | Init(c,s) :: ForkConsistency(c, s)
+    ensures forall c, s, s' | ForkConsistency(c, s) && Next(c, s, s') :: ForkConsistency(c, s')
+{
+}
+
+// this predicate and the following lemma are a way to prevent trivial
+// specifications of the problem that would prevent a philosopher from
+// having both forks
+predicate PhilosopherHasBothForks(c:Constants, s:State, pi:nat)
+    requires pi < c.tableSize
+    requires WellFormed(c, s)
+{
+    && s.philosophers[pi].left
+    && s.philosophers[pi].right
+}
+
+lemma PseudoLiveness(c:Constants, pi:nat) returns (b:seq<State>)
+    requires c.tableSize == 3
+    requires pi == 1
+    ensures 0 < |b| 
+    ensures Init(c, b[0])
+    ensures forall i | 0 <= i < |b|-1 :: Next(c, b[i], b[i+1])
+    ensures WellFormed(c, b[|b|-1])
+    ensures PhilosopherHasBothForks(c, b[|b|-1], pi)
+{
+    var s0 := State([Pair(false,false), Pair(false, false), Pair(false, false)]);
+    var s1 := State([Pair(false,false), Pair(true, false), Pair(false, false)]);
+    var s2 := State([Pair(false,false), Pair(true, true), Pair(false, false)]);
+    assert AcquireLeft(c, s0, s1, 1); // witness
+    assert AcquireRight(c, s1, s2, 1); // witness
+    b := [s0, s1, s2];
+}
+
